platform/cito/ElimDead.v
@@ -1,0 +1,8 @@
+Set Implicit Arguments.
+
+Fixpoint elim_dead s :=
+  match s with
+    | Skip => Skip
+    | a ;; b => 
+      let result := elim_dead b in
+      
